verify_body_sound

bin/rust/rocq/AxSem.v
@@ -250,7 +250,7 @@ Definition wp_Body
     (Q: Value -> iProp Σ)
     : iProp Σ :=
   ∀ (env: Env),
-  ⌜ ∀ x info, assoc x (local_decls body) = Some info → (env x).1 = ty info ⌝ -∗
+  ⌜ ∀ x info, assoc x (local_decls body) = Some info → ty info = (env x).1 ⌝ -∗
   ⌜ ∀ x, (env x).2 ≠ null_ptr ⌝ -∗
   ⌜ Forall (λ '(x, info), assoc x (local_decls body) = Some info) (local_decls body) ⌝ -∗ (* Local variable names are unique *)
   match local_decls body with
